Proper euclidian division def, with the proof that quotient/modulo behave right. Using new tactics not commited yet to do patterns on contexts/sigmas.

Basics.v
@@ -1,5 +1,63 @@
-Require Export Program Equations Have.
+Require Export Arith Program Equations Have.
 
 Hint Extern 4 => discriminates : core.
 
 Ltac simpdep := reverse ; simplify_dep_elim ; simplify_IH_hyps.
+
+Definition ltb (x y : nat) := leb (S x) y.
+
+Program Fixpoint euclid (n : nat) (m : nat) `{Have (m > 0)} {wf lt n} : nat * nat :=
+  match ltb n m with
+    | true => (0, n)
+    | false => let '(q, r) := euclid (n - m) m return nat * nat in
+      (S q, r)
+  end.
+
+  Next Obligation.
+    unfold ltb in *.
+    symmetry in Heq_anonymous.
+    apply leb_complete_conv in Heq_anonymous. unfold Have in *. omega.
+  Qed.
+
+  Next Obligation. auto with *. Defined.
+
+Ltac ind_on f := 
+  match goal with
+    |- context [ f ?x ] => let term := fresh "term" in 
+      pattern_tele x term ; pattern_call (f term) ; subst term ;
+        apply Fix_sub_rect ; fold f ; unfold MR in * ; simpl ; intros
+  end.
+
+Lemma euclid_spec n m `{Have (m > 0)} : forall q r, euclid n m = (q, r) -> n = m * q + r.
+Proof.
+  intros n m H. unfold euclid. ind_on euclid_func. 
+  admit.
+
+  destruct x as [ n' [ m' Hm' ] ]; simpl in *.
+  case_eq (ltb n' m') ; intro Hlt ; rewrite Hlt in *. 
+  program_simpl. omega.
+  match type of H1 with
+    context [ euclid_func ?t ] => specialize (H0 t)
+  end.
+  simpl in H0.
+  destruct_call euclid_func.
+  program_simpl.
+  apply leb_complete_conv in Hlt.
+  assert(n' - m' < n') by (unfold Have in * ; omega).
+  specialize (H0 H1).
+  simplify_IH_hyps. replace (m' * S n0 + r) with (m' + (m' * n0 + r)) by ring.
+  rewrite <- H0.
+  rewrite <- le_plus_minus. reflexivity.
+  omega.
+Defined.
+
+Eval compute in (euclid 66 8).
+
+Definition quotient_nat n m `{Have (m > 0)} : nat := fst (euclid n m).
+Definition modulo_nat n m `{Have (m > 0)} : nat := snd (euclid n m).
+
+Lemma quotient_cancel : forall x y `{Have (y > 0)}, modulo_nat x y = 0 -> quotient_nat x y * y = x.
+Proof. intros x y H. unfold modulo_nat, quotient_nat in *. 
+  generalize (euclid_spec x y). destruct_call euclid ; intros Heucl ; simplify_IH_hyps.
+  simpl in *. intros. subst. ring.
+Defined.
